>[!note] Change of Basis
>Let $\{\vec{v}_1, \vec{v}_2, \dots, \vec{v}_n \}$ be a V-[[2.8a Basis|basis]] (nonstandard basis) of $\mathbb{R}^n$. Let $\vec{x}$ be a vector given in the standard basis. The representation of $\vec{x}$ in the V-basis is
>$$\vec{z} = V^{-1}\vec{x},$$
>where $V := \begin{bmatrix}\vec{v}_1 & \vec{v}_2 & \dots & \vec{v}_n\end{bmatrix}$ is an invertible square basis matrix.

# Intuition
Think of it this way: we can translate a vector $\vec{z}$ in V-basis to $\vec{x}$ in our basis using a matrix $V$ that contains the representation in our basis of what V-basis members see as their standard basis ($\left\{\begin{bmatrix}1 \\ 0\end{bmatrix},\begin{bmatrix}0 \\ 1\end{bmatrix}\right\}$). Suppose V-basis unit vectors $\vec{v}_1$ and $\vec{v}_2$ can be translated into standard basis using our unit vectors as $\vec{v}_1=2\vec{e}_1+3\vec{e}_2$  and $\vec{v}_2=\vec{e}_1-2\vec{e}_2$. Therefore, the V-basis matrix representation in our (standard) basis is $V=\begin{bmatrix}\vec{v}_1 & \vec{v}_2\end{bmatrix}=\begin{bmatrix}2 & 1 \\ 3 & -2\end{bmatrix}$. Algebraically, we can convert a V-basis vector $\vec{z}=\begin{bmatrix}3 \\ 2\end{bmatrix}=3\vec{v}_1+2\vec{v}_2$ to our basis as $\vec{x}=3(2\vec{e}_1+3\vec{e}_2)+2(\vec{e}_1-2\vec{e}_2)=8\vec{e}_1+5\vec{e}_2=\begin{bmatrix}8 \\ 5\end{bmatrix}.$ We can quickly verify this by equivalently solving $\vec{x}=\begin{bmatrix}2 & 1 \\ 3 & -2\end{bmatrix}\begin{bmatrix}3 \\ 2\end{bmatrix}=3\begin{bmatrix}2 \\ 3\end{bmatrix}+2\begin{bmatrix}1 \\ -2\end{bmatrix}=\begin{bmatrix}8 \\ 5\end{bmatrix}$. Then, in order to reverse the process, we redo it backwards (by taking the inverse). 

### Why do we take the inverse to translate to V-basis?
Think of it in the following way: the way people using V-basis see our basis is $V^{-1}=\begin{bmatrix}\frac{2}{7} & \frac{1}{7} \\ \frac{3}{7} & -\frac{2}{7}\end{bmatrix}$. For them, $\vec{e}_1 = \frac{2}{7}\vec{v}_1 + \frac{3}{7}\vec{v}_2=$ and $\vec{e}_2 = \frac{1}{7}\vec{v}_1 -\frac{2}{7}\vec{v}_2$. We can quickly verify this by running our representations of the V-basis vectors $\vec{v}_1$ and $\vec{v}_2$ to find out that $\vec{e}_1=\begin{bmatrix}1 \\ 0\end{bmatrix}$ and $\vec{e}_2=\begin{bmatrix}0 \\ 1\end{bmatrix}$. Therefore, our vector $\vec{x}=\begin{bmatrix}8 \\ 5\end{bmatrix}=\begin{bmatrix}1 & 0 \\ 0 & 1\end{bmatrix}\begin{bmatrix}8 \\ 5\end{bmatrix}=8\vec{e}_1+5\vec{e}_2$ can be written in V-basis as $\vec{z}=8\left(\frac{2}{7}\vec{v}_1+\frac{3}{7}\vec{v}_2\right)+5\left(\frac{1}{7}\vec{v}_1+-\frac{2}{7}\vec{v}_2\right)=\frac{16}{7}\vec{v}_1+\frac{24}{7}\vec{v}_2+\frac{5}{7}\vec{v}_1-\frac{10}{7}\vec{v}_2=3\vec{v}_1+2\vec{v}_2=\begin{bmatrix}3 \\ 2\end{bmatrix}$. This can also be verified by solving $\vec{z}=\begin{bmatrix}\frac{2}{7} & \frac{1}{7} \\ \frac{3}{7} & -\frac{2}{7}\end{bmatrix}\begin{bmatrix}8 \\ 5\end{bmatrix}=8\begin{bmatrix}\frac{2}{7} \\ \frac{3}{7}\end{bmatrix}+5\begin{bmatrix}\frac{1}{7} \\ -\frac{2}{7}\end{bmatrix}=\begin{bmatrix}3 \\ 2\end{bmatrix}$.

### How can we find the inverse coefficients algebraically?
Consider our main example where $\vec{v}_1=2\vec{e}_1+3\vec{e}_2$  and $\vec{v}_2=\vec{e}_1-2\vec{e}_2$. We can solve for the representations of $\vec{e}_1$ and $\vec{e}_2$ in V-basis such that 
$$
\begin{dcases}
	\vec{e}_1=\vec{v}_2+2\vec{e}_2 \\
	\vec{e}_1=\frac{1}{2}\vec{v}_1-\frac{3}{2}\vec{e}_2
\end{dcases}
\iff
\frac{7}{2}\vec{e}_2=\frac{1}{2}\vec{v}_1-\vec{v}_2
\iff
\begin{dcases}
\vec{e}_1 = \frac{2}{7}\vec{v}_1+\frac{3}{7}\vec{v}_2\\
\vec{e}_2 = \frac{1}{7}\vec{v}_1-\frac{2}{7}\vec{v}_2
\end{dcases}.
$$
We can verify that this is true by substituting for the respective values of $\vec{v}_1$ and $\vec{v}_2$. As such, our standard basis vectors are represented in V-basis as $\left\{\begin{bmatrix}\frac{2}{7}\\ \frac{3}{7}\end{bmatrix},\begin{bmatrix}\frac{1}{7} \\ -\frac{2}{7}\end{bmatrix}\right\}$. 

Why does this equal $V^{-1}$?