>[!note] Modular Inverse
>An integer $x$ has a ***unique*** multiplicative inverse $y$ [[4.1 Modulo|modulo]] $m$ if and only if $\gcd(x, m)=1$, such that
>$$x \cdot y \equiv 1 \pmod{m}.$$
# Proof
1. Let's start with the simple fact that if $\gcd(x, m)=1$, then $x$ and $m$ are coprime, meaning that 1 is the greatest common number that divides them. This is crucial because if $x$ and $m$ were not coprime, then they would both be multiples of some integer $d \geq 1$, so the definition of modulo $xy=1+qm$ cannot hold, because $xy$ and $qm$ are both multiples of $d$ for any $y,q$, but $1+qm$ is not, as $d \geq 1$.
2. Now, consider the set of $m$ distinct remainders $R=\{0, 1, \dots, m-1\}$. Notice now that $Rx=\{0, x,\dots,(m-1)x\}$ is still distinct, and therefore $R \equiv Rx \pmod{m}$. It follows that there is only one unique integer $a \pmod{m}$ in $R$ for which $ax \equiv 1 \pmod{m}$. If there was more than one such integer, this would break the set $R$ and the laws of modular arithmetic. We can also proceed by contradiction for a stronger proof:
	- Suppose there are two numbers $a,b \in R$, such that $a \geq b$ and $ax \equiv bx \pmod{m}$. Then, $(a-b)x \equiv 0 \pmod{m}$, or by congruence $(a-b)x=km$, meaning that $m$ divides $(a-b)x$ into some integer $k \in \mathbb{Z}$. However, since $x$ and $m$ are coprime, then $(a-b)$ must be a multiple of $m$ equal to $k \geq 1$, but by definition $0 \leq a-b \leq m-1$ is always less than $m$, so $(a-b)x=km$ cannot hold.

# Examples
> [!example] Multiplicative Inverse of $(n-1) \pmod{n}$
> We need to find the multiplicative inverse $x$, such that
> $$(n-1)x \equiv 1 \pmod{n}.$$
> We can do so by expanding the equation, such that
> $$
>\begin{align}
>(n-1)x &\equiv (xn-x) \pmod{n}\\ 
>&\equiv 0-x \pmod{n}\\ 
>&\equiv 1 \pmod{n}
>\end{align}
> $$
>Logically, $-x \equiv 1 \pmod{n} \iff x \equiv -1 \pmod{n}$. In the standard modular range $\{0, \ldots, n-1\}$, $-1 \equiv n-1 \pmod{n}$. As such,
>$$x \equiv n-1 \pmod{n}.$$
>We can verify that this is correct as follows:
>$$
>\begin{align}
>(n-1)^2 &\equiv n^2-2n+1 \pmod{n}\\
>&\equiv 0-0+1 \pmod{n}\\
>&\equiv 1 \pmod{n}
\end{align}
>$$

