>[!note] Solving Bezout's Identity
>We can compute the [[4.4a Modular Inverse|inverse]] of an integer modulo $m$ $x \in \mathbb{Z}$ as $y$ by solving Bezout's identity ($ax+by=d=\gcd(x, y)$) for the case of $d=1$, such that
>$$am+xy=1,$$
>where $m \in \mathbb{N}$ and $a \in \mathbb{Z}$. We can do so using the extended Euclidean algorithm, which returns the factor $d$, as well as the coefficients $a,b$ of Bezout's identity:
>```run-python
>def extended_gcd(x, y):
>	if y == 0:
>		print((x, 1, 0))
>		return (x, 1, 0)
>	else:
>		(d, a, b) = extended_gcd(y, x % y)
>		print((d, b, a - (x // y) * b))
>		return (d, b, a - (x // y) * b)
>		
>extended_gcd(19, 4)
>```
>The algorithm takes $O(n)$ time.

# Understanding
The case of Bezout's identity for $d=1$ means that our two integers $x$ and $m$ are coprime. This satisfies the condition for the existence a modular inverse of $x$, $y$ (modulo $m$), such that $xy \equiv 1 \pmod{m}$. As such, we can find two integers $a,y \in \mathbb{Z}$ such that $am+xy=1$.

The extended Euclid's algorithm follows the principle of the original EA that if $x \geq y > 0$, then $\gcd(x,y)=\gcd(y, x \pmod{y})$. It returns $d$ in the place of $x$ of the initial call, in the form of $\gcd(d, 0)$. However, the extended algorithm also utilizes Bezout's identity to compute the coefficients $a$ and $b$. 

Let's take a look at Bezout's identity once again: $d=Ax+By$. In the base case ($n$-th recursion), where $y_n=0$, $d=x_n$ as per the vanilla algorithm, the equation holds for $A_n=1$ and $B_n=0$, since $d=1 \cdot x_n+0 \cdot y_n$. Then, $d$ remains constant at $x_n$ throughout the rest of the recursion.

However, for the $k$-th recursive call where $y_k>0$ for $k \in [1, n)$, we need to first receive the tuple from the $(k+1)$-th recursive step and employ the division algorithm (see 4.1) with backward substitution to compute the values $A_k, B_k$ from $A_{k+1}, B_{k+1}$ such that for the $k$-th step, $d=A_kx_k+B_ky_k=A_{k+1}x_{k+1} + B_{k+1}x_{k+1} \pmod{y_{k+1}})$ holds. This is because by definition of EA, $x_{k+1}=y_k$ and $y_{k+1}=x_k \pmod{y_k}$. Note that we are now going backwards, such that the ($k+1$)-th  step precedes the $k$-th step, which could be a bit confusing:
$$
\begin{align}
d &= A_{k+1}x_{k+1} + B_{k+1}y_{k+1} \\
&= A_{k+1}y_k+B_{k+1}(x_k \pmod{y_k}) \\
&= A_{k+1}y_k+B_{k+1}(x_k - \lfloor \frac{x_k}{y_k} \rfloor y_k) \\
&= B_{k+1}x_k+(A_{k+1}-\lfloor \frac{x_k}{y_k} \rfloor B_{k+1})y_k.
\end{align}
$$
The final step is a result of factoring out $x_k$ and $y_k$, and by inspection $A_k=B_{k+1}$ and $B_k=A_{k+1}-\lfloor \frac{x_k}{y_k} \rfloor B_{k+1}$ for $k \in [1, n)$, which is exactly how the coefficients are calculated in the algorithm.
# Properties
##### *(Eucl. Alg.)* For two integers $x,y \in \mathbb{N}$ such that $x \geq y > 0$, $\gcd(x,y)=gcd(y, x \pmod{y)}$.
- We can verify this by writing $x=qy+r$ where $q=\lfloor \frac{x}{y} \rfloor$ and $r=x \pmod{y}$. Then, if $d=\gcd(x,y)$ is the greatest common divisor (e.g. divides both $x$ and $y$), then naturally it will also divide $x$ and $qy$, and therefore it divides their difference $r=x-qy=x \pmod{y}$ (see examples of 1. for proof).
##### *(Divisibility)* For three integers $x,y,z \in \mathbb{N}$ such that $\gcd(x,y)=1$, if $x \mid yz$, then $x \mid z$.
- This can be seen by inspection; if $x$ cannot divide $y$ but divides $yz$, then it must divide $z$. 
- We can also utilize extended Euclid for a stronger proof: there are integers $A,B \in \mathbb{Z}$ such that $Ax+By=1=\gcd(x,y)$. Multiplying both sides by $z$ gives us $Axz+Byz=z$. Then, $x \mid Axz$ since it is a multiple of $x$. Also, since by definition $x \mid yz$, then $x \mid Byz$. Thus, logically, $x$ also divides their sum ($x \mid Axz + Byz$). Since $z=Axz+Byz$, then $x \mid z$.
# Example
>[!example] Finding the Inverse of $16 \pmod{9}$
>If we wanted to find the inverse $y$ of $16 \pmod{9}$, such that $16y \equiv 1 \pmod{9}$, we would find by inspection that $y \equiv 4 \pmod{9}$ satisfies our solution such that $28 \equiv 1 \pmod{9}$. We can illustrate the algorithm in the following table:
>
>|  $n$  | $x$ | $m$ | $d$ | $a$ | $y$ |
>| :---: | :-: | :-: | :-: | :-: | :-: |
>| **1** | 16  |  9  |  1  |  4  | -7  |
>| **2** |  9  |  7  |  1  | -3  |  4  |
>| **3** |  7  |  2  |  1  |  1  | -3  |
>| **4** |  2  |  1  |  1  |  0  |  1  |
>| **5** |  1  |  0  |  1  |  1  |  0  |
>This result is also given by running the code above.